src/theories/Mod_Simp.thy
@@ -60,13 +60,13 @@ fun has_mod rng m s =
 
 fun pull_mod rng cmod cm ct =
   if Thm.term_of cm aconv Thm.term_of ct then
-    Drule.instantiate' [SOME (Thm.ctyp_of_cterm ct)] [SOME ct]
+    Thm.instantiate' [SOME (Thm.ctyp_of_cterm ct)] [SOME ct]
       @{thm mod_self_cong}
   else if has_mod rng (Thm.term_of cm) (Thm.term_of ct) then
     case Thm.term_of ct of
       Const (@{const_name mod}, _) $ _ $ _ =>
         let val (cx, cm) = Thm.dest_binop ct
-        in Drule.instantiate' [SOME (Thm.ctyp_of_cterm cx)] [SOME cx, SOME cm]
+        in Thm.instantiate' [SOME (Thm.ctyp_of_cterm cx)] [SOME cx, SOME cm]
           @{thm mod_mod_trivial}
         end
     | Const (@{const_name plus}, _) $ _ $ _ =>
@@ -86,7 +86,7 @@ fun pull_mod rng cmod cm ct =
         end
     | Const (@{const_name power}, _) $ _ $ _ =>
         let val (cl, cr) = Thm.dest_binop ct
-        in Drule.instantiate' [] [NONE, NONE, NONE, SOME cr]
+        in Thm.instantiate' [] [NONE, NONE, NONE, SOME cr]
           @{thm power_mod_cong} OF [pull_mod rng cmod cm cl]
         end
     | Const (@{const_name uminus}, _) $ _ =>
@@ -94,21 +94,16 @@ fun pull_mod rng cmod cm ct =
         in @{thm minus_mod_cong} OF [pull_mod rng cmod cm cu] end
     | _ => raise Fail "pull_mod"
   else
-    Drule.instantiate' [SOME (Thm.ctyp_of_cterm ct)]
+    Thm.instantiate' [SOME (Thm.ctyp_of_cterm ct)]
       [SOME (Drule.list_comb (cmod, [ct, cm]))] refl;
 
 fun pull_mod_proc _ ctxt ct = (case Thm.term_of ct of
     Const (@{const_name mod}, Type (_, [T, _])) $ u $ m =>
       let val rng = Sign.of_sort
         (Proof_Context.theory_of ctxt)
-        (T, @{sort ring})
+        (T, @{sort ring_div})
       in
-        if
-          Sign.of_sort
-            (Proof_Context.theory_of ctxt)
-            (T, @{sort semiring_div}) andalso
-          has_mod rng m u
-        then
+        if has_mod rng m u then
           let val (cmod, [cu, cm]) = Drule.strip_comb ct
           in SOME (mk_meta_eq (pull_mod rng cmod cm cu)) end
         else NONE
