src/theories/lsc-bignum/lscmnbignum_Lsc__bignum__equal__subprogram_def_WP_parameter_def_1.thy
@@ -5,18 +5,13 @@ begin
 why3_open "lscmnbignum_Lsc__bignum__equal__subprogram_def_WP_parameter_def_1.xml"
 
 why3_vc WP_parameter_def
-proof -
-  from `o1 \<le> a_last` `\<not> o1 + 1 \<le> a_last`
-  have "o1 = a_last" by simp
-  with
+  using
     `mk_bool__ref True = mk_bool__ref result_us`
     `(result_us = _) = _`
-    `(if (if elts a o1 = elts b (b_first + (o1 - a_first)) then _
+    `(if (if elts a a_last = elts b (b_first + (a_last - a_first)) then _
       else _) \<noteq> _ then _ else _) \<noteq> _`
     `a_first \<le> a_last`
-  show ?thesis
-    by (simp add: num_of_lint_equals_iff word32_to_int_lower word32_to_int_upper')
-qed
+  by (simp add: num_of_lint_equals_iff word32_to_int_lower word32_to_int_upper')
 
 why3_end
 
