src/theories/lsc-bignum/lscmnbignum_Lsc__bignum__equal__subprogram_def_WP_parameter_def_2.thy
@@ -5,17 +5,12 @@ begin
 why3_open "lscmnbignum_Lsc__bignum__equal__subprogram_def_WP_parameter_def_2.xml"
 
 why3_vc WP_parameter_def
-proof -
-  from `o1 \<le> a_last` `\<not> o1 + 1 \<le> a_last`
-  have "o1 = a_last" by simp
-  with
+  using
     `mk_bool__ref result_us = mk_bool__ref result_us1`
     `(result_us1 = _) = _`
     `(num_of_big_int' a _ _ = num_of_big_int' b _ _) = _`
-  show ?thesis
-    by (simp add: num_of_lint_equals_iff uint_lt [where 'a=32, simplified]
-      word32_to_int_def del: num_of_lint_sum)
-qed
+  by (simp add: num_of_lint_equals_iff uint_lt [where 'a=32, simplified]
+    word32_to_int_def del: num_of_lint_sum)
 
 why3_end
 
