src/theories/lsc-bignum/lscmnbignum_Lsc__bignum__less__subprogram_def_WP_parameter_def_3.thy
@@ -6,11 +6,11 @@ why3_open "lscmnbignum_Lsc__bignum__less__subprogram_def_WP_parameter_def_3.xml"
 
 why3_vc WP_parameter_def
 proof -
-  let ?l' = "i - a_first"
-  let ?l = "1 + (a_last - i)"
+  let ?l' = "o1 - a_first"
+  let ?l = "1 + (a_last - o1)"
   let ?a' = "int_of_math_int (num_of_big_int' a a_first ?l')"
   let ?b' = "int_of_math_int (num_of_big_int' b b_first ?l')"
-  let ?a = "int_of_math_int (num_of_big_int' a i ?l)"
+  let ?a = "int_of_math_int (num_of_big_int' a o1 ?l)"
   let ?b = "int_of_math_int (num_of_big_int' b (b_first + ?l') ?l)"
   let ?c = "Base ^ nat ?l'"
   have "0 \<le> ?a'"
@@ -22,14 +22,13 @@ proof -
   moreover from
     `(num_of_big_int' a _ _ = num_of_big_int' b _ _) = _`
     `_ = (if BV32.ult (elts a o1) (elts b _) then _ else _)`
-    `mk_int__ref i = mk_int__ref o1` `o1 \<le> a_last`
+    `o1 \<le> a_last`
   have "?a < ?b" by (simp add: word32_to_int_def BV32.ult_def)
   ultimately have "?a' + ?c * ?a < ?b' + ?c * ?b"
     by (rule msw_less)
   then have "int_of_math_int (num_of_big_int' a a_first (?l' + ?l)) <
     int_of_math_int (num_of_big_int' b b_first (?l' + ?l))"
     using `a_first \<le> o1` `o1 \<le> a_last`
-      `mk_int__ref i = mk_int__ref o1` [simplified]
     by (simp only: num_of_lint_sum) simp
   then show ?thesis by (simp add: sign_simps)
 qed
