src/theories/lsc-bignum/lscmnbignum_Lsc__bignum__less__subprogram_def_WP_parameter_def_4.thy
@@ -6,12 +6,10 @@ why3_open "lscmnbignum_Lsc__bignum__less__subprogram_def_WP_parameter_def_4.xml"
 
 why3_vc WP_parameter_def
 proof -
-  from `a_first \<le> o1` `\<not> a_first \<le> o1 - 1`
-  have "o1 = a_first" by simp
-  with
+  from
     `(num_of_big_int' a _ _ = num_of_big_int' b _ _) = _`
-    `(if BV32.ugt (elts a o1) (elts b _) then True else False) \<noteq> True`
-    `(if BV32.ult (elts a o1) (elts b _) then True else False) \<noteq> True`
+    `(if BV32.ugt (elts a a_first) (elts b _) then True else False) \<noteq> True`
+    `(if BV32.ult (elts a a_first) (elts b _) then True else False) \<noteq> True`
     `a_first \<le> a_last`
   have "num_of_big_int' a a_first (1 + (a_last - a_first)) =
     num_of_big_int' b b_first (1 + (a_last - a_first))"
