src/theories/lsc-bignum/lscmnbignum_Lsc__bignum__mont_exp__subprogram_def_WP_parameter_def_11.thy
@@ -23,8 +23,6 @@ proof -
     `(num_of_big_int' (Array aux32 _) _ _ = _) = _`
     `(num_of_big_int' (Array (aux1(aux1_first := o1)) _) _ _ = _) = _`
     `e_first \<le> e_last`
-    `\<not> e_first \<le> i1 - 1` `e_first \<le> i1`
-    `\<not> 0 \<le> j2 - 1` `0 \<le> j2`
   have "num_of_big_int (word32_to_int o a) a_first ?L =
     ?x ^ nat (num_of_big_int (word32_to_int \<circ> elts e) e_first (1 + (e_last - e_first))) *
     (Base * minv ?m Base mod ?m) ^ nat ?L mod ?m"
