src/theories/lsc-bignum/lscmnbignum_Lsc__bignum__mont_exp__subprogram_def_WP_parameter_def_12.thy
@@ -1,0 +1,41 @@
+theory lscmnbignum_Lsc__bignum__mont_exp__subprogram_def_WP_parameter_def_12
+imports "../LibSPARKcrypto"
+begin
+
+why3_open "lscmnbignum_Lsc__bignum__mont_exp__subprogram_def_WP_parameter_def_12.xml"
+
+why3_vc WP_parameter_def
+proof -
+  let ?L = "a_last - a_first + 1"
+  let ?m = "num_of_big_int (word32_to_int \<circ> elts m) m_first ?L"
+  let ?x = "num_of_big_int (word32_to_int \<circ> elts x) x_first ?L"
+  let ?r = "num_of_big_int (word32_to_int \<circ> elts r) r_first ?L"
+  let ?R = "Base ^ nat ?L"
+  note m_inv = `of_int 1 + m_inv * elts m m_first = of_int 0`
+    [simplified word_uint_eq_iff uint_word_ariths, simplified,
+     folded word32_to_int_def]
+
+  from `a_first < a_last` `(_ < num_of_big_int' m _ _) = _` [simplified]
+  have Base_inv: "Base * minv ?m Base mod ?m = 1"
+    by (simp only: lint_inv_mod [of "\<lfloor>m_inv\<rfloor>\<^sub>s" "word32_to_int o elts m" _ 32, simplified, OF m_inv])
+
+  from `(num_of_big_int' r  _ _ = _) = _`
+    [unfolded base_eq, simplified math_int_conv math_int_of_int_inv]
+  have "?r * minv ?m Base ^ nat ?L mod ?m =
+    (?R * (Base * minv ?m Base mod ?m) ^ nat ?L) mod ?m"
+    by (simp only: nat_mult_distrib power_mult power_mult_distrib
+        power2_eq_square [simplified transfer_nat_int_numerals])
+      (simp add: power_mult_distrib mult.assoc)
+  then have R: "?r * minv ?m Base ^ nat ?L mod ?m = ?R mod ?m"
+    by (simp add: Base_inv)
+
+  from `(num_of_big_int' (Array aux2 _) _ _ = _) = _`
+  have "num_of_big_int (word32_to_int o aux2) aux2_first ?L =
+    ?x * (?r * minv ?m Base ^ nat ?L mod ?m) mod ?m"
+    by (simp add: mult.assoc base_eq)
+  with R show ?thesis by (simp add: base_eq)
+qed
+
+why3_end
+
+end
