src/theories/lsc-bignum/lscmnbignum_Lsc__bignum__mont_exp_window__subprogram_def_WP_parameter_def_38.thy
@@ -51,8 +51,8 @@ proof -
       BV64.ule_def word_of_int uint_word_of_int natural_in_range_def
       mod_pos_pos_trivial)
   also from i `BV64.ule (of_int j2) i1`
-    `elts e (e_first + uint ((i1 - of_int j2) div of_int 32)) AND
-     of_int 2 ^ nat (uint ((i1 - of_int j2) mod of_int 32)) \<noteq> of_int 0`
+    `_ = (elts e (e_first + uint ((i1 - of_int j2) div of_int 32)) AND
+     of_int 2 ^ nat (uint ((i1 - of_int j2) mod of_int 32)) \<noteq> of_int 0)`
     uint_lt [of i1]
     `_ \<longrightarrow> natural_in_range j2`
   have "?e AND 2 ^ nat (uint i1 - j2) \<noteq> 0"
