src/theories/lsc-bignum/lscmnbignum_Lsc__bignum__mont_exp_window__subprogram_def_WP_parameter_def_64.thy
@@ -22,27 +22,24 @@ proof -
       [of "\<lfloor>m_inv\<rfloor>\<^sub>s" "word32_to_int o elts m" _ 32, simplified, OF m_inv]
       del: num_of_lint_sum)
 
-  from `h2 \<le> r214b` `\<not> h2 + 1 \<le> r214b`
-  have "h2 = r214b" by simp
-
   from
     `\<forall>k. \<lfloor>aux3__first\<rfloor>\<^sub>\<int> \<le> k \<and> k \<le> \<lfloor>aux3__last\<rfloor>\<^sub>\<int> \<longrightarrow> _`
     `\<lfloor>aux3__first\<rfloor>\<^sub>\<int> \<le> aux3_first`
     `aux3_first + (a_last - a_first) \<le> \<lfloor>aux3__last\<rfloor>\<^sub>\<int>`
-  have "num_of_big_int (word32_to_int o aux32) aux3_first ?L =
+  have "num_of_big_int (word32_to_int o aux31) aux3_first ?L =
     num_of_big_int (word32_to_int o a2) a_first ?L"
     by (simp add: num_of_lint_ext add_diff_eq)
   also from
     `(num_of_big_int' (Array a2 _) _ _ = _) = _`
     `(math_int_from_word w = _) = _`
   have "num_of_big_int (word32_to_int o a2) a_first ?L =
-    num_of_big_int (word32_to_int \<circ> aux33) aux3_first ?L *
+    num_of_big_int (word32_to_int \<circ> aux32) aux3_first ?L *
     num_of_big_int (word32_to_int \<circ> aux4)
       (aux4_first + ?e div 2 ^ nat (uint i1 - (r214b - 1)) mod
        2 ^ nat r214b div 2 * ?L) ?L * minv ?m Base ^ nat ?L mod ?m"
     by (simp add: ediv_def base_eq BV32.facts.to_uint_lsr [of _ 1, simplified])
-  also note `(num_of_big_int' (Array aux33 _) _ _ = _) = _`
-    [simplified `h2 = r214b` base_eq, simplified]
+  also note `(num_of_big_int' (Array aux32 _) _ _ = _) = _`
+    [simplified base_eq, simplified]
   also {
     have "?e div 2 ^ nat (uint i1 - (r214b - 1)) mod 2 ^ nat r214b < 2 ^ nat r214b"
       by simp
