src/theories/lsc-bignum/lscmnbignum_Lsc__bignum__mont_exp_window__subprogram_def_WP_parameter_def_74.thy
@@ -1,0 +1,18 @@
+theory lscmnbignum_Lsc__bignum__mont_exp_window__subprogram_def_WP_parameter_def_74
+imports "../LibSPARKcrypto"
+begin
+
+why3_open "lscmnbignum_Lsc__bignum__mont_exp_window__subprogram_def_WP_parameter_def_74.xml"
+
+why3_vc WP_parameter_def
+proof -
+  from `1 \<le> h1` `a_first < a_last`
+  have "0 \<le> h1 * (a_last - a_first + 1)"
+    by simp
+  with `\<lfloor>aux4__first\<rfloor>\<^sub>\<int> \<le> aux4_first` `a_first < a_last`
+  show ?thesis by simp
+qed
+
+why3_end
+
+end
