src/theories/lsc-bignum/lscmnbignum_Lsc__bignum__mont_mult__subprogram_def_WP_parameter_def_1.thy
@@ -7,8 +7,7 @@ why3_open "lscmnbignum_Lsc__bignum__mont_mult__subprogram_def_WP_parameter_def_1
 why3_vc WP_parameter_def
   using
     `\<forall>k. a_first \<le> k \<and> k \<le> a_last \<longrightarrow> a k = of_int 0`
-    `(math_int_from_word (of_int 1) < num_of_big_int' m _ _) = True`
-  by (simp_all add: num_of_lint_all0 word32_to_int_def)
+  by (simp add: num_of_lint_all0 word32_to_int_def)
 
 why3_end
 
