src/theories/lsc-bignum/lscmnbignum_Lsc__bignum__mont_mult__subprogram_def_WP_parameter_def_3.thy
@@ -5,16 +5,12 @@ begin
 why3_open "lscmnbignum_Lsc__bignum__mont_mult__subprogram_def_WP_parameter_def_3.xml"
 
 why3_vc WP_parameter_def
-proof -
-  from `\<not> i1 + 1 \<le> a_last` `i1 \<le> a_last`
-  have "i1 = a_last" by simp
-  with `(if less _ _ _ _ _ \<noteq> _ then _ else _) \<noteq> _`
+  using
+    `(if less _ _ _ _ _ \<noteq> _ then _ else _) \<noteq> _`
     `(less _ _ _ _ _ = _) = _`
     `((num_of_big_int' (Array a _) _ _ + _) mod _ = _) = _`
-  show ?thesis
-    by (simp add: base_eq mod_pos_pos_trivial
-      num_of_lint_lower word32_to_int_lower diff_add_eq)
-qed
+  by (simp add: base_eq mod_pos_pos_trivial
+    num_of_lint_lower word32_to_int_lower diff_add_eq)
 
 why3_end
 
