src/theories/lsc-bignum/lscmnbignum_Lsc__bignum__shr_inplace__subprogram_def_WP_parameter_def_3.thy
@@ -5,15 +5,11 @@ begin
 why3_open "lscmnbignum_Lsc__bignum__shr_inplace__subprogram_def_WP_parameter_def_3.xml"
 
 why3_vc WP_parameter_def
-proof -
-  from `mk_int__ref i = mk_int__ref (i1 - 1)` `\<not> a_first \<le> i1 - 1` `a_first \<le> i1`
-  have "i1 = a_first" by simp
-  with
+  using
+    `mk_int__ref i = mk_int__ref a_first`
     `(num_of_big_int' (Array a2 _) _ _ = num_of_big_int' (Array a1 _) _ _ * _ + _) = _`
     `mk_map__ref a = mk_map__ref a1`
-  show ?thesis
-    by (simp add: diff_diff_eq2 diff_add_eq zdiv_zadd1_eq)
-qed
+  by (simp add: diff_diff_eq2 diff_add_eq zdiv_zadd1_eq)
 
 why3_end
 
