src/theories/lsc-bignum/lscmnbignum_Lsc__bignum__size_square_mod__subprogram_def_WP_parameter_def_6.thy
@@ -5,15 +5,10 @@ begin
 why3_open "lscmnbignum_Lsc__bignum__size_square_mod__subprogram_def_WP_parameter_def_6.xml"
 
 why3_vc WP_parameter_def
-proof -
-  from `\<not> j + 1 \<le> 63` `j \<le> 63`
-  have "j = 63" by simp
-  with
-    `(num_of_big_int' (Array r2 _) _ _ = _) = _`
+  using
+    `(num_of_big_int' (Array r1 _) _ _ = _) = _`
     `m_first \<le> i1`
-  show ?thesis
-    by (simp add: diff_add_eq [symmetric] nat_add_distrib mult_ac base_eq)
-qed
+  by (simp add: diff_add_eq [symmetric] nat_add_distrib mult_ac base_eq)
 
 why3_end
 
