src/theories/lsc-bignum/lscmnbignum_Lsc__bignum__size_square_mod__subprogram_def_WP_parameter_def_7.thy
@@ -5,18 +5,12 @@ begin
 why3_open "lscmnbignum_Lsc__bignum__size_square_mod__subprogram_def_WP_parameter_def_7.xml"
 
 why3_vc WP_parameter_def
-proof -
-  from `\<not> j2 + 1 \<le> 63` `j2 \<le> 63`
-  have "j2 = 63" by simp
-  moreover from `\<not> i1 + 1 \<le> m_last` `i1 \<le> m_last`
-  have "i1 = m_last" by simp
-  ultimately show ?thesis using
+  using
     `mk_map__ref r = mk_map__ref r1`
     `mk_map__ref r1 = mk_map__ref r2`
     `(num_of_big_int' (Array r2 _) _ _ = _) = _`
     `m_first \<le> m_last`
-    by (simp add: nat_add_distrib mult_ac base_eq)
-qed
+  by (simp add: nat_add_distrib mult_ac base_eq)
 
 why3_end
 
