src/theories/lsc-bignum/lscmnbignum_Lsc__bignum__word_inverse__subprogram_def_WP_parameter_def_5.thy
@@ -6,8 +6,8 @@ why3_open "lscmnbignum_Lsc__bignum__word_inverse__subprogram_def_WP_parameter_de
 
 why3_vc WP_parameter_def
   using
-    `of_int (gcd (uint (p2 * m)) (uint (of_int 0))) = of_int 1`
-    `mk_t__ref p = mk_t__ref p2`
+    `of_int (gcd (uint (p * m)) (uint (of_int 0))) = of_int 1`
+    `mk_t__ref p1 = mk_t__ref p`
   by (simp add: word_of_int)
 
 why3_end
