src/theories/lsc-ripemd160/lscmnripemd160_Lsc__ripemd160__hash_context__subprogram_def_WP_parameter_def_3.thy
@@ -7,25 +7,21 @@ why3_open "lscmnripemd160_Lsc__ripemd160__hash_context__subprogram_def_WP_parame
 why3_vc WP_parameter_def
 proof -
   from `dynamic_invariant3 message True False True`
-    `BV64.ule (unsigned_64_to_rep (first (rt message)))
-       (unsigned_64_to_rep (last (rt message)))`
+    `BV64.ule (first (rt message)) (last (rt message))`
   have first: "uint (first (rt message)) \<le> 36028797018963967"
     and last: "uint (last (rt message)) \<le> 36028797018963967"
     by (simp_all add: dynamic_invariant3_def dynamic_property_def
-      BV64.ule_def in_range2_def first1_def last1_def
-      unsigned_64_to_rep_def)
+      BV64.ule_def in_range2_def first1_def last1_def)
   from `ucast (length1 mod of_int 512) \<noteq> of_int 0`
   have "length1 mod 512 \<noteq> 0" by auto
   with uint_lt [of length1] uint_0 [of length1]
     `BV64.ule (length1 div _ + _) _`
-    `BV64.ule (unsigned_64_to_rep (first (rt message)))
-       (unsigned_64_to_rep (last (rt message)))`
+    `BV64.ule (first (rt message)) (last (rt message))`
     diff_mono [OF uint_0 [of "first (rt message)"] last]
-    `BV64.ule (unsigned_64_to_rep (first (rt message)))
-       (unsigned_64_to_rep (last (rt message)))`
+    `BV64.ule (first (rt message)) (last (rt message))`
   have length:
     "uint (length1 div 512) \<le> uint (last (rt message)) - uint (first (rt message))"
-    by (simp add: unsigned_64_to_rep_def
+    by (simp add:
       BV64.ule_def [folded word_le_def] length_def first1_def last1_def
       trans [OF fun_cong [OF word_of_int] word_of_int_uint]
       word_le_def uint_word_ariths uint_div mod_pos_pos_trivial
@@ -34,7 +30,7 @@ proof -
     [OF length, of "uint (first (rt message))", simplified]
     last]
   show ?thesis
-    by (simp add: BV64.ule_def unsigned_64_to_rep_def uint_word_ariths
+    by (simp add: BV64.ule_def uint_word_ariths
       mod_pos_pos_trivial)
 qed
 
